Strips/VarSet.lean
@@ -1,0 +1,196 @@
+module
+
+public import Mathlib.Data.SetLike.Basic
+
+public section
+
+namespace STRIPS
+
+/-!
+# Sets of Variables
+
+This file implements set of variables with the aim to be both easy to work with and effient at
+runtime.
+-/
+
+/-! ## Sets of variables
+
+Variables have type `Fin n`, where `n` is the number of variables.
+Sets of variables are internally represented by a bitvector of length `n`.
+-/
+structure VarSet (n : ℕ) where
+  toBitVec : BitVec n
+deriving DecidableEq, Repr
+
+namespace VarSet
+
+instance {n} : SetLike (VarSet n) (Fin n) where
+  coe V := { i | V.toBitVec[i] }
+
+  coe_injective := by
+    rintro ⟨V⟩ ⟨V'⟩
+    simp only [Fin.getElem_fin, Set.ext_iff, Set.mem_setOf_eq, Bool.coe_iff_coe, Fin.forall_iff,
+      mk.injEq, BitVec.eq_of_getElem_eq_iff, imp_self]
+
+lemma mem_iff {n i} {V : VarSet n} : i ∈ V ↔ V.toBitVec[i] := by
+  unfold SetLike.instMembership
+  simp only [SetLike.coe, Set.mem_setOf_eq]
+
+instance {n} {i : Fin n} {V : VarSet n} : Decidable (i ∈ V) := by
+  rw [mem_iff]
+  infer_instance
+
+@[reducible]
+instance {n} : HasSubset (VarSet n) where
+  Subset V V' := ∀ i ∈ V, i ∈ V'
+
+instance {n} : EmptyCollection (VarSet n) where
+  emptyCollection := ⟨BitVec.zero n⟩
+
+@[simp]
+lemma mem_empty {n i} : i ∉ (∅ : VarSet n) := by
+  unfold instEmptyCollection
+  simp [mem_iff]
+
+def insert {n} (i : Fin n) (V : VarSet n) : VarSet n :=
+  ⟨V.toBitVec ||| BitVec.twoPow n i⟩
+
+@[simp]
+lemma mem_insert {n} {V : VarSet n} {i j} : j ∈ (V.insert i) ↔ j ∈ V ∨ j = i := by
+  simp [insert, mem_iff]
+  grind
+
+/-- Return the `VarSet` containing all variables in the given list. -/
+def ofList {n} (l : List (Fin n)) : VarSet n :=
+  l.foldr insert ∅
+
+@[simp]
+lemma mem_ofList {n} {l : List (Fin n)} {i} : i ∈ (ofList l) ↔ i ∈ l := by
+  simp only [ofList]
+  induction l with
+  | nil => simp only [List.foldr_nil, mem_empty, List.not_mem_nil]
+  | cons j l ih =>
+    grind only [List.mem_cons, = List.foldr_cons, mem_insert]
+
+instance {n} : Union (VarSet n) where
+  union V V' := ⟨V.toBitVec ||| V'.toBitVec⟩
+
+@[simp]
+lemma mem_union {n} {V V' : VarSet n} {i} : i ∈ V ∪  V' ↔ i ∈ V ∨ i ∈ V' := by
+  unfold instUnion
+  simp [mem_iff]
+
+@[simp]
+lemma empty_union {n} {V : VarSet n} : ∅ ∪ V = V := by
+  simp only [SetLike.ext_iff, mem_union, mem_empty, false_or, implies_true]
+
+@[simp]
+lemma union_empty {n} {V : VarSet n} : V ∪ ∅ = V := by
+  simp only [SetLike.ext_iff, mem_union, mem_empty, or_false, implies_true]
+
+instance {n} : Inter (VarSet n) where
+  inter V V' := ⟨V.toBitVec &&& V'.toBitVec⟩
+
+@[simp]
+lemma mem_inter {n} {V V' : VarSet n} {i} : i ∈ V ∩ V' ↔ i ∈ V ∧ i ∈ V' := by
+  unfold instInter
+  simp [mem_iff]
+
+@[simp]
+lemma empty_inter {n} {V : VarSet n} : ∅ ∩ V = ∅ := by
+  simp only [SetLike.ext_iff, mem_inter, mem_empty, false_and, implies_true]
+
+@[simp]
+lemma inter_eq_empty_iff {n} {V V' : VarSet n} : V ∩ V' = ∅ ↔ ∀ i ∈ V, i ∉ V' := by
+  simp only [SetLike.ext_iff, mem_inter, mem_empty, iff_false, not_and]
+
+instance {n} : Compl (VarSet n) where
+  compl V := ⟨~~~V.toBitVec⟩
+
+@[simp]
+lemma mem_compl {n} {V : VarSet n} {i} : i ∈ Vᶜ ↔ i ∉ V := by
+  unfold instCompl
+  simp [mem_iff]
+
+instance {n} : SDiff (VarSet n) where
+  sdiff V V' := ⟨V.toBitVec &&& ~~~V'.toBitVec⟩
+
+@[simp]
+lemma mem_diff {n} {V V' : VarSet n} {i} : i ∈ V \ V' ↔ i ∈ V ∧ i ∉ V' := by
+  unfold instSDiff
+  simp [mem_iff]
+
+/--
+Folds a function over all variables in `V` with starting value `init`. The variables are combined
+in increasing order.
+-/
+def foldl {α n} (f : α → Fin n → α) (init : α) (V : VarSet n) : α :=
+  Fin.foldl n (fun a i ↦ if i ∈ V then f a i else a) init
+
+lemma foldl_cons {α n} {V : VarSet n} {f : Fin n → α} {a as} :
+    a ∈ V.foldl (fun a i ↦ f i :: a) as ↔ (∃ i ∈ V, a = f i) ∨ a ∈ as := by
+  simp only [foldl]
+  rcases V with ⟨V⟩
+  induction V using BitVec.cons_induction with
+  | nil => simp
+  | @cons n' b V ih =>
+    simp only [mem_iff, Fin.getElem_fin, Fin.foldl_succ_last, Fin.val_last,
+      Fin.val_castSucc] at *
+    have h1 : ∀ i : Fin n', i.val ≠ n' := by omega
+    split
+    · simp only [BitVec.getElem_cons, h1, ↓reduceDIte, List.mem_cons, ih]
+      constructor
+      · grind
+      · rw [← or_assoc]
+        apply Or.imp_left
+        rintro ⟨i, h2, rfl⟩
+        split at h2
+        · grind
+        · apply Or.inr
+          use ⟨i.val, by omega⟩
+          simp [h2]
+    · simp only [BitVec.getElem_cons, h1, ↓reduceDIte, ih]
+      constructor
+      · grind
+      · apply Or.imp_left
+        rintro ⟨i, h2, rfl⟩
+        split at h2
+        · grind
+        · use ⟨i.val, by omega⟩
+          simp [h2]
+
+-- TODO : can this be done more efficiently?
+def map {n m} (V : VarSet n) (f : Fin n → Fin m) : VarSet m :=
+  V.foldl (fun V' i ↦ V'.insert (f i)) ∅
+  -- Fin.foldl n (fun V' i ↦ if i ∈ V then V'.insert (f i) else V') empty
+
+lemma mem_map {n m} {V : VarSet n} {f : Fin n → Fin m} {i} :  i ∈ V.map f ↔ (∃ j ∈ V, i = f j) := by
+  simp only [map, foldl, insert]
+  rcases V with ⟨V⟩
+  induction V using BitVec.cons_induction with
+  | nil => simp
+  | @cons n' b V ih =>
+    simp only [mem_iff, Fin.getElem_fin, Fin.foldl_succ_last, Fin.val_last,
+      Fin.val_castSucc] at *
+    have h1 : ∀ i : Fin n', i.val ≠ n' := by omega
+    split
+    · simp only [BitVec.getElem_cons, h1, ↓reduceDIte, BitVec.getElem_or, BitVec.getElem_twoPow,
+      Bool.or_eq_true, ih, decide_eq_true_eq]
+      constructor
+      · grind
+      · rintro ⟨i, h2, rfl⟩
+        split at h2
+        · grind
+        · apply Or.inl
+          use ⟨i.val, by omega⟩
+          simp [h2]
+    · simp only [BitVec.getElem_cons, h1, ↓reduceDIte, ih]
+      constructor
+      · grind
+      · rintro ⟨i, h2, rfl⟩
+        split at h2
+        · grind
+        · use ⟨i.val, by omega⟩
+          simp [h2]
+
+end STRIPS.VarSet
